src/program_proof/wal/recovery_proof.v
@@ -2,11 +2,13 @@ From RecordUpdate Require Import RecordSet.
 
 From Perennial.program_proof Require Import disk_lib.
 From Perennial.program_proof Require Import wal.invariant.
+From Perennial.program_proof Require Import wal.circ_proof_crash.
 
 Section goose_lang.
 Context `{!heapG Σ}.
 Context `{!lockG Σ}.
 Context `{!walG Σ}.
+Context `{!crashG Σ}.
 
 Implicit Types (v:val) (z:Z).
 Implicit Types (γ: wal_names (Σ:=Σ)).
@@ -26,15 +28,68 @@ Theorem wp_MkLog_init d (bs: list Block) :
 Proof.
 Admitted.
 
-(* this seems odd - will it really be able to recover the circular log from this
-assumption? how do we make this assumption modular? *)
-Theorem wp_MkLog_recover l0 d γ σ :
-  {{{ is_wal_inner l0 γ σ ∗ is_circular circN (circular_pred γ) γ.(circ_name) }}}
-    MkLog #d
+Theorem wpc_mkLog_recover stk k E1 E2 d γ σ :
+  {{{ is_wal_inner_durable γ σ }}}
+    mkLog #d @ stk; k; E1; E2
   {{{ σ' γ' l, RET #l;
       ⌜relation.denote (log_crash) σ σ' tt⌝ ∗
-      is_wal_inner l γ' σ' ∗ is_circular circN (circular_pred γ') γ'.(circ_name) }}}.
+       is_wal_inv_pre l γ' σ' ∗
+       (* XXX whatever it is that background threads needs *)
+       True}}}
+  {{{ ∃ γ', is_wal_inner_durable γ' σ }}}.
 Proof.
-Admitted.
+  clear P.
+  iIntros (Φ Φc) "Hcs HΦ".
+  rewrite /mkLog.
+
+  Ltac show_crash1 := eauto.
+
+  wpc_pures; first by show_crash1.
+  iNamed "Hcs".
+  iNamed "Hdisk".
+  wpc_bind (recoverCircular _).
+
+  Ltac show_crash2 :=
+    try (crash_case); iExists _;
+    iSplitL ""; first auto;
+    iFrame; iExists _, _, _; iFrame; iFrame "#".
+
+  wpc_apply (wpc_recoverCircular with "[$]").
+  iSplit.
+  { iIntros "Hcirc". show_crash2. }
+
+  iNext. iIntros (γ' c diskStart diskEnd bufSlice upds).
+  iIntros "(Hupd_slice&Hcirc&Happender&Hstart&Hdisk&%&%)".
+
+  wpc_frame_compl "Hupd_slice".
+  { crash_case. iExists (set circ_name (λ _, γ') γ). destruct γ.
+    rewrite /is_wal_inner_durable. simpl. rewrite /is_durable_txn/is_installed_txn/is_durable//=.
+    simpl. iSplitL ""; first auto. rewrite /txns_ctx.
+    (* XXX: need to somehow show that all of these predicates do not depend on the circ_name... *)
+    admit.
+  }
+  (* XXX: these tuples are parenthesized the wrong way for these projections *)
+  wp_pure _.
+  wp_pure _.
+  wp_pure _.
+  wp_pure _.
+  wp_pure _.
+  wp_pure _.
+  wp_pures.
+  iDestruct "Hupd_slice" as (?) "(Hbufsloc&Hupds)".
+  (* How can end be the Fst of #bufSlice.(Slice.cap) which appears
+     to be a u64 ??? *)
+Abort.
+
+
+Theorem wpc_MkLog_recover stk k E1 E2 d γ σ :
+  {{{ is_wal_inner_durable γ σ }}}
+    MkLog #d @ stk; k; E1; E2
+  {{{ σ' γ' l, RET #l;
+      ⌜relation.denote (log_crash) σ σ' tt⌝ ∗
+       is_wal_inv_pre l γ' σ' }}}
+  {{{ ∃ γ', is_wal_inner_durable γ' σ }}}.
+Proof.
+Abort.
 
 End goose_lang.
